Remove requirement in ApplyReductionPlanToBehavior that states must be empty, make easier-to-satisfy post-condition on lemma_UpdatePerformIosToHostNext

ironfleet/src/Dafny/Distributed/Concur/RemoveUpdates.i.dfy
@@ -3,7 +3,6 @@ include "RefinementConvolution.i.dfy"
 include "SystemRefinement.i.dfy"
 include "ReductionPlan.i.dfy"
 include "MatchTreesToTrace.i.dfy"
-include "../Common/Collections/Maps.i.dfy"
 
 module RemoveUpdatesModule {
 
@@ -12,70 +11,6 @@ module RemoveUpdatesModule {
     import opened SystemRefinementModule
     import opened ReductionPlanModule
     import opened MatchTreesToTraceModule
-    import opened Collections__Maps_i
-
-    function RemoveActorStatesFromSystemState(ls:SystemState) : SystemState
-    {
-        ls.(states := map[])
-    }
-
-    lemma lemma_SystemCorrespondenceBetweenSystemStateAndItselfWithoutActorStates(
-        ls:SystemState,
-        hs:SystemState
-        )
-        requires hs == RemoveActorStatesFromSystemState(ls);
-        ensures  SystemCorrespondence(ls, hs);
-        ensures  SystemCorrespondence(hs, ls);
-        decreases |ls.states|;
-    {
-        if ls.states == map [] {
-            return;
-        }
-
-        var actor :| actor in ls.states;
-        var new_states := RemoveElt(ls.states, actor);
-        var ms := ls.(states := new_states);
-        var relation := GetSystemSystemRefinementRelation();
-        lemma_SystemCorrespondenceBetweenSystemStateAndItselfWithoutActorStates(ms, hs);
-        assert RefinementPair(ms, hs) in relation;
-        assert RefinementPair(hs, ms) in relation;
-
-        forall ss | SpecCorrespondence(ms, ss)
-            ensures SpecCorrespondence(ls, ss);
-        {
-            var entry := Entry(actor, UpdateLocalState());
-            assert SystemNextEntry(ls, ms, entry);
-            lemma_LeftMoverBackwardPreservation(entry, ls, ms, ss);
-        }
-        assert SystemCorrespondence(ls, ms);
-        assert RefinementPair(ls, ms) in relation;
-
-        forall ss | SpecCorrespondence(ls, ss)
-            ensures SpecCorrespondence(ms, ss);
-        {
-            var entry := Entry(actor, UpdateLocalState());
-            assert SystemNextEntry(ls, ms, entry);
-            lemma_RightMoverForwardPreservation(entry, ls, ms, ss);
-        }
-        assert SystemCorrespondence(ms, ls);
-        assert RefinementPair(ms, ls) in relation;
-
-        lemma_SystemRefinementRelationConvolvesWithItself();
-        assert RefinementPair(ls, hs) in relation;
-    }
-
-    lemma lemma_SystemCorrespondenceBetweenSystemStatesDifferingOnlyInActorStates(
-        ls:SystemState,
-        hs:SystemState
-        )
-        requires hs == ls.(states := hs.states);
-        ensures  SystemCorrespondence(ls, hs);
-    {
-        var ms := RemoveActorStatesFromSystemState(ls);
-        lemma_SystemCorrespondenceBetweenSystemStateAndItselfWithoutActorStates(ls, ms);
-        lemma_SystemCorrespondenceBetweenSystemStateAndItselfWithoutActorStates(hs, ms);
-        lemma_SystemRefinementRelationConvolvesWithItself();
-    }
 
     lemma lemma_SystemNextEntryPreservedWhenRemovingActorState(
         ls0:SystemState,
